theories/iris/examples/segstack/function/segstack_push.v
@@ -1,0 +1,568 @@
+From mathcomp Require Import ssreflect eqtype seq ssrbool.
+From iris.program_logic Require Import language.
+From iris.proofmode Require Import base tactics classes.
+From iris.base_logic Require Export gen_heap ghost_map proph_map na_invariants.
+From iris.base_logic.lib Require Export fancy_updates.
+From iris.bi Require Export weakestpre.
+Require Export segstack_common segstack_is_full iris_fundamental proofmode.
+
+Set Implicit Arguments.
+Unset Strict Implicit.
+Unset Printing Implicit Defensive.
+
+
+
+Section stack.
+  Context `{!wasmG Σ, HHB: HandleBytes}.
+  
+  Section code.
+
+(*
+  push: [handle, i32] -> []
+  locals declared: [i32]
+
+  Given a stack pointer and an i32, push the i32 to the top of the stack.
+
+  Implementation contains the is_full check which results in a trap if the stack is full. Otherwise, load the 
+  stack top pointer from the stack pointer address, increment it by 4, store the given i32 to the new cell and 
+  update the stack top pointer. Does not cause u32 overflow when the stack pointer is at the last page 
+  of memory.
+  
+  Returns nothing. Can trap only if the stack pointer is invalid or the stack is full.
+
+  Parameters/Locals:
+  0 (input)     stack pointer
+  1 (input)     i32 value to be pushed
+  2             temporary variable storing the new address of the stack top pointer
+*)
+    Definition push_op :=
+      is_full_op ++ 
+     [
+       BI_if (Tf [] []) [BI_unreachable] [];
+       BI_get_local 0 ;
+       BI_segload T_i32;
+       i32const 4 ;
+       BI_binop T_i32 (Binop_i BOI_add) ;
+       BI_tee_local 2 ;
+       BI_get_local 0 ;
+       BI_handleadd ;
+       BI_get_local 1 ;
+       BI_segstore T_i32;
+       BI_get_local 0 ;
+       BI_get_local 2 ;
+       BI_segstore T_i32 
+      ].
+        
+    Definition push :=
+      (*validate_stack 0 ++ validate_stack_bound 0 ++*) push_op.
+    
+  End code.
+
+  Section specs.
+    
+    Lemma spec_push_op f0 (v: handle) (a : i32) s E :
+      ⊢ {{{ 
+           ⌜ f0.(f_locs) !! 0 = Some (value_of_handle v) ⌝
+          ∗ ⌜ f0.(f_locs) !! 1 = Some (VAL_int32 a) ⌝ 
+          ∗ ⌜ length f0.(f_locs) >= 3 ⌝
+          ∗ ⌜ (N.of_nat (length s) < two14 - 1)%N ⌝
+          ∗ isStack v s
+          ∗ ↪[frame] f0 }}}
+        to_e_list push_op @ E
+        {{{ w, ⌜ w = immV [] ⌝ ∗
+                       isStack v (a :: s) ∗
+                       ∃ f1, ↪[frame] f1 ∗ ⌜ f_inst f0 = f_inst f1 ⌝ }}}. 
+    Proof.
+      iIntros "!>" (Φ) "(%Hlocv & %Hloca & %Hlocs & %Hlens & Hstack & Hf) HΦ" => /=.
+      
+      iDestruct (stack_pure with "Hstack") as "(%Hoff & %Hbound & %Hvalid & %Hlen)".
+      
+      rewrite (separate4 (AI_basic _)).
+      iApply wp_seq.
+      iSplitR; last iSplitL "Hf Hstack".
+      2: { iApply (spec_is_full_op with "[$Hf $Hstack] []") => //.
+           iIntros (w) "H".
+           by iApply "H".
+      }
+      { iIntros "H".
+        by iDestruct "H" as (k) "(%Habs & ?)".
+      }           
+
+      iIntros (w) "H".
+      iDestruct "H" as (k) "(-> & Hstack & %Hret & Hf)".
+      destruct Hret as [Hret | Hret] => //.
+      { destruct Hret as [-> Hlens'].
+        rewrite Hlens' in Hlens. lia.
+      }
+
+      destruct Hret as [-> _] => /=.
+
+      rewrite separate2.
+      iApply wp_seq.
+      instantiate (1 := λ w, (⌜ w = immV [ ]⌝ ∗ ↪[frame] f0)%I).
+      iSplitR; first by iIntros "(%H & _)".
+      iSplitL "Hf".
+      iApply (wp_if_false with "Hf") => //.
+      { iIntros "!> Hf".
+        take_drop_app_rewrite 0.
+        iApply (wp_block with "Hf") => //.
+        iIntros "!> Hf /=".
+        by iApply (wp_label_value with "Hf").
+      }
+
+      iIntros (w) "(-> & Hf)" => /=.
+
+      rewrite (separate1 (AI_basic _)).
+      iApply wp_seq.
+      
+      instantiate (1 := λ x, (⌜ x = immV _ ⌝ ∗ ↪[frame] f0)%I).
+      iSplitR ; first by iIntros "[%Habs _]".
+      iSplitL "Hf".
+      - iApply (wp_get_local with "[] [$Hf]") => //=.
+      - iIntros (w) "[-> Hf]".
+        simpl.
+        rewrite separate2.
+        iApply wp_seq.
+        instantiate ( 1 := λ x, ((⌜ x = immV [value_of_uint (N.of_nat (length s) * 4)] ⌝ ∗ isStack v s ∗ ↪[frame] f0)%I)).
+        iSplitR ; first by iIntros "(%Habs & _)".
+        iSplitR "HΦ".
+        { by iApply (stack_load_0 with "[$] [$]") => //. }
+
+      - iIntros (w) "(-> & Hstack & Hf)" => /=.
+        rewrite separate3.
+        iApply (wp_seq _ _ _ (λ x, (⌜ x = immV [value_of_uint (4 + N.of_nat (length s) * 4)] ⌝
+                                            ∗ ↪[frame] _)%I)).
+        iSplitR ; first by iIntros "[%Habs _]".
+        iSplitL "Hf".
+        iApply (wp_binop with "Hf") => //.
+        iIntros "!>".
+        iPureIntro.
+        unfold value_of_int, value_of_uint => /=.
+        repeat f_equal.
+        unfold Wasm_int.Int32.iadd, Wasm_int.Int32.add => /=.
+        f_equal.
+        rewrite Wasm_int.Int32.Z_mod_modulus_eq.
+        rewrite Z.mod_small ; first by lias.
+        rewrite u32_modulus. unfold two14 in Hlen. 
+        remember (length s) as x.
+        rewrite -Heqx.
+        by lias. 
+      - iIntros (w) "[-> Hf]".
+        simpl.
+        rewrite separate2.
+        iApply wp_seq; iSplitR; last iSplitL "Hf".
+        instantiate (1 := λ w, (⌜ w = immV [value_of_uint (4 + N.of_nat (length s) * 4)] ⌝ ∗ ↪[frame] _) %I).
+        2: {
+             iApply (wp_tee_local with "Hf").
+             iIntros "!> Hf".
+             rewrite separate1.
+             iApply wp_val_app => //.
+             iSplitR; first by iIntros "!> [%Habs _]".
+             iApply (wp_set_local with "[] [$Hf]") => //=.
+        }
+        { by iIntros "(%Habs & _)". }
+        
+      - iIntros (w) "[-> Hf]".
+        iSimpl.
+
+        remember {| f_locs := set_nth (value_of_uint (4 + N.of_nat (length s) * 4))
+                                (f_locs f0) 2 (value_of_uint (4 + N.of_nat (length s) * 4)) ;
+                   f_inst := f_inst f0 |} as f1.
+        rewrite - Heqf1.
+        rewrite separate2.
+        iApply wp_seq.
+        instantiate (1 := λ x, (⌜ x = immV _ ⌝ ∗ ↪[frame] _)%I).
+        iSplitR; first by iIntros "[% _]".
+        iSplitL "Hf".
+      - rewrite separate1. iApply wp_val_app => //.
+        iSplitR; first by iIntros "!> [% _]".
+        subst f1; iApply (wp_get_local with "[] [$Hf]") => //=.
+        rewrite - fmap_insert_set_nth; last lia.
+        rewrite list_lookup_insert_ne => //.
+      - iIntros (w) "[-> Hf]".
+        iSimpl.
+        rewrite separate3.
+        iApply wp_seq.
+        instantiate (1 := λ x, (⌜ x = immV _ ⌝ ∗ ↪[frame] _)%I).
+        iSplitR; first by iIntros "[% _]".
+        iSplitL "Hf".
+      - iApply (wp_handleadd with "Hf") => //.
+        unfold handle_add.
+        assert (0 <= Z.of_N (offset v) +
+     Wasm_int.Z_of_sint i32m
+       (Wasm_int.int_of_Z i32m (Z.of_N (4 + N.of_nat (length s) * 4))))%Z.
+        simpl. rewrite wasm_int_signed. lia. unfold two14 in Hlen.
+        remember (length s) as x. rewrite - Heqx. lia.
+        apply Z.geb_le in H. rewrite H. done.
+      - iIntros (w) "[-> Hf]".
+        iSimpl.
+        rewrite separate2.
+        iApply wp_seq.
+        instantiate (1 := λ x, (⌜ x = immV _ ⌝ ∗ ↪[frame] f1)%I).
+        iSplitR ; first by iIntros "[%Habs _]".
+        iSplitL "Hf".
+      - rewrite separate1.
+        iApply wp_val_app => //.
+        iSplitR ; first by iIntros "!> [%Habs _]".
+        subst f1 ; iApply (wp_get_local with "[] [$Hf]") => //.
+        simpl.
+        rewrite - fmap_insert_set_nth; last by lias.
+        rewrite list_lookup_insert_ne => //.
+      - iIntros (w) "[-> Hf]".
+        iSimpl.
+        rewrite separate3.
+        iApply wp_seq.
+        instantiate (1 := λ x, (⌜ x = immV [] ⌝ ∗ (
+        ↦[i32][ base v] Wasm_int.Int32.repr (Z.of_N (N.of_nat (length s) * 4)) ∗
+        (([∗ list] i↦w ∈ s, 
+                            ↦[i32][ base v + N.of_nat (length s) * 4 -
+                                    4 * N.of_nat i] w) ∗
+         (∃ (bs: seq.seq (byte * btag)), ⌜ N.of_nat (length bs) = (two16 - 4 - N.of_nat (length s) * 4 - 4)%N ⌝ ∗ [∗ list] k↦y ∈ bs, ↦[ws][N.of_nat
+                                               (N.to_nat
+                                                  (base v + N.of_nat (length s) * 4 +
+                                                  4) +
+                                                  (4 + k))]y)) ∗
+        (* [∗ list] k↦y ∈ bs,  ↦[ws][N.of_nat
+                                      (N.to_nat (base v + N.of_nat (length s) * 4 + 4) +
+                                       S (S (S (S k))))]y ∗ *)
+                               id v↣[allocated](base v, bound v) ∗
+        ↦[wss][base v +
+                  Z.to_N
+                    (Z.of_N (offset v) +
+                     Wasm_int.Int32.signed
+                       (Wasm_int.Int32.repr (Z.of_N (4 + N.of_nat (length s) * 4))))] 
+        map (λ b : byte, (b, Numeric)) (bits (VAL_int32 a)) ∗  ↪[frame]f1))%I). 
+        iSplitR ; first by iIntros " [%Habs _]". 
+        iDestruct "Hstack" as "(_ & _ & _ & _ & Hid & Hbase & Hs & Hrest)".
+        iDestruct "Hrest" as (bs) "[%Hbs Hrest]".
+        unfold two16 in Hbs.
+        unfold two14 in Hlens.
+        remember (length s) as x.
+        rewrite - Heqx.
+        assert ((65536-4-N.of_nat x * 4)%N >= 4)%N as Hlen'; first lia.
+        do 4 (destruct bs; first by exfalso; rewrite - Hbs in Hlen'; lias).
+        rewrite separate4.
+        unfold seg_block_at_pos at 1.
+        rewrite big_sepL_app.
+        iDestruct "Hrest" as "[Ha Hrest]".
+        iSplitR "HΦ".
+      - iApply wp_wand_r. iSplitL. iApply wp_segstore ; last first.
+        iFrame.
+        iSplitR "Ha".
+        iNext.
+        iCombine "Hbase Hs Hrest" as "H".
+        instantiate (1 := λ x, (⌜ x = immV [] ⌝ ∗ _)%I).
+        iSplit => //.
+        iExact "H". 
+        4: by instantiate (1 := [p; p0; p1; p2]).
+        4: done.
+        3: done.
+        3: done.
+        iApply (big_sepL_impl with "Ha").
+        iIntros "!>" (k y) "% H".
+        rewrite of_nat_to_nat_plus.
+        simpl.
+        rewrite wasm_int_signed; last lia. 
+        unfold handle_addr => /=.
+        rewrite Z2N.inj_add.
+        rewrite N2Z.id. rewrite N2Z.id.
+        rewrite Nat2N.inj_add. rewrite N2Nat.id.
+        rewrite Hoff. rewrite N.add_0_l.
+        rewrite (N.add_comm 4 (_ * 4)).
+        rewrite N.add_assoc. done. lia. lia.
+        simpl. rewrite Hoff Hbound. rewrite wasm_int_signed; last lia.
+        lia.
+
+      - iIntros (w) "(((-> & H0 & H1 & H1') & H2 & H2') & H3)".
+        iSplit => //. 
+        iFrame.  
+        iExists bs.
+        iSplit; last by iFrame.
+        unfold two16.
+        repeat rewrite cons_length in Hbs.
+        remember (length bs) as x'.
+        iPureIntro.
+        lia.
+        
+      - iIntros (w) "(-> & H)".
+        iDestruct "H" as "(Hbase & (Hs & Hrest) & Hid & Ha & Hf)".
+        iSimpl.
+        rewrite (separate1 (AI_basic _)).
+        iApply wp_seq.
+        instantiate (1 := λ x, ( ⌜ x = immV _ ⌝ ∗ ↪[frame]f1)%I).
+        iSplitR ; first by iIntros "[%Habs _]".
+        iSplitL "Hf".
+      - iApply (wp_get_local with "[] [$Hf]") => //.
+        subst f1 => //.
+        rewrite - fmap_insert_set_nth; last by lias.
+        by rewrite list_lookup_insert_ne => //.
+          
+      - iIntros (w) "[-> Hf]".
+        iSimpl.
+        rewrite separate2.
+        iApply wp_seq.
+        instantiate (1 := λ x, ( ⌜ x = immV _ ⌝
+                                         ∗ ↪[frame] f1)%I).
+        iSplitR ; first by iIntros "[%Habs _]".
+        iSplitL "Hf".
+      - rewrite separate1.
+        iApply wp_val_app => //.
+        iSplitR ; first by iIntros "!> [%Habs _]".
+        iApply (wp_get_local with "[] [$Hf]") => //.
+        subst f1 => //.
+        rewrite set_nth_read => //=.
+                  
+      - iIntros (w) "[-> Hf]".
+        iSimpl.
+        iApply wp_wand_r.
+        iSplitL "Hf Hbase Hid".
+      - iApply wp_segstore; last first => //. 
+        iFrame. instantiate (2 := λ x, ⌜ x = immV _ ⌝%I). iSplit => //.
+        iApply i32_wss. unfold handle_addr; rewrite Hoff N.add_0_r. done.
+        rewrite Hoff Hbound. simpl. lia. done.
+      - iIntros (w) "[(-> & Hid & Hbase) Hf]".
+        iApply "HΦ".
+        iSplit => //.
+        unfold isStack.
+        iSplitR "Hf"; last by iExists f1; subst f1; iFrame.
+        repeat iSplit => //.
+        iPureIntro => /= ; rewrite - Heqx ; clear Heqx s ; unfold two14 ; lia.
+        iSplitL "Hid"; first done.
+        iSplitL "Hbase".
+        iApply i32_wss. unfold handle_addr; rewrite Hoff N.add_0_r.
+        simpl.
+        rewrite - Heqx.
+        replace (Z.of_N (4 + N.of_nat x * 4)) with (Z.pos (Pos.of_succ_nat x * 4)).
+        done. lia.
+        
+        iSplitR "Hrest".
+        iSplitL "Ha".
+        iApply i32_wss => //=.
+        rewrite wasm_int_signed; last lia.
+        rewrite Hoff. rewrite Z.add_0_l.
+        rewrite N2Z.id. rewrite - Heqx.
+        rewrite N.sub_0_r.
+        replace (4 + N.of_nat x * 4)%N with (N.pos (Pos.of_succ_nat x * 4)); last lia.
+        done.
+        
+        iApply (big_sepL_impl with "Hs").
+        iIntros "!>" (k y) "%Hbits H".
+        iApply (points_to_i32_eq with "H") => //.
+        rewrite cons_length - Heqx.
+        lia.
+        
+        iDestruct "Hrest" as (bs0) "(%Hbslen & Hrest)".
+        iExists bs0.
+        iSplit => //.
+        iPureIntro.
+        rewrite cons_length.
+        repeat rewrite cons_length in Hbs.
+        rewrite - Heqx.
+        lias.
+        rewrite cons_length -Heqx.
+        unfold seg_block_at_pos.
+        iApply (big_sepL_impl with "Hrest").
+        iIntros "!>" (k y) "%Hl Hy".
+        do 2 rewrite of_nat_to_nat_plus.
+        assert (base v + N.of_nat x * 4 + 4 + N.of_nat (4 + k) =
+                  base v + N.of_nat (S x) * 4 + 4 + N.of_nat k)%N.
+        lia. rewrite H.  done.
+    Qed.
+
+    (*
+    Lemma spec_push f0 n (v: N) (a : i32) s E :
+      ⊢ {{{ ⌜ f0.(f_inst).(inst_memory) !! 0 = Some n ⌝
+          ∗ ⌜ f0.(f_locs) !! 0 = Some (value_of_uint v) ⌝
+          ∗ ⌜ f0.(f_locs) !! 1 = Some (VAL_int32 a) ⌝ 
+          ∗ ⌜ length f0.(f_locs) >= 3 ⌝
+         ∗ ⌜ (N.of_nat (length s) < two14 - 1)%N ⌝
+          ∗ isStack v s n
+          ∗ ↪[frame] f0 }}}
+        to_e_list push @ E
+        {{{ w, ⌜ w = immV [] ⌝ ∗
+                       isStack v (a :: s) n ∗
+                       ∃ f1, ↪[frame] f1 ∗ ⌜ f_inst f0 = f_inst f1 ⌝ }}}. 
+    Proof.
+      iIntros "!>" (Φ) "(%Hinst & %Hlocv & %Hloca & %Hlocs & %Hlens & Hstack & Hf) HΦ" => /=.
+      
+      rewrite separate4.
+      iApply wp_seq.
+      instantiate (1 := λ x,  (⌜ x = immV [] ⌝ ∗ isStack v s n ∗ ↪[frame] f0)%I).
+      iSplitR; first by iIntros "(%H & _)".
+      iSplitL "Hstack Hf"; first by iApply (is_stack_valid with "[$Hstack $Hf]").
+      
+      iIntros (w) "(-> & Hstack & Hf) /=".
+      rewrite separate3.
+      iApply wp_seq.
+      instantiate (1 := λ x,  (⌜ x = immV [] ⌝ ∗ isStack v s n ∗ ↪[frame] f0)%I).
+      iSplitR; first by iIntros "(%H & _)".
+      iSplitL "Hstack Hf"; first by iApply (is_stack_bound_valid with "[$Hstack $Hf]").
+      
+      iIntros (w) "(-> & Hstack & Hf) /=".
+      iApply (spec_push_op with "[$Hf $Hstack] [$]").
+      auto.
+    Qed. *)
+      
+  End specs.
+
+
+  Section valid.
+    Context `{!logrel_na_invs Σ}.
+    Set Bullet Behavior "Strict Subproofs".
+(*
+    Lemma valid_push m t funcs :
+    let i0 := {| inst_types := [Tf [] [T_i32]; Tf [T_i32] [T_i32]; Tf [T_i32; T_i32] []];
+                     inst_funcs := funcs;
+                     inst_tab := [t];
+                     inst_memory := [m];
+                     inst_globs := []
+              |} in
+    na_inv logrel_nais stkN (stackModuleInv (λ (a : N) (b : seq.seq i32), isStack a b m) (λ n : nat, N.of_nat m↦[wmlength]N.of_nat n)) -∗
+    interp_closure_native i0 [T_i32;T_i32] [] [T_i32] (to_e_list push) [].
+  Proof.
+    iIntros "#Hstk".
+    iIntros (vcs f) "#Hv Hown Hf".
+    iIntros (LI HLI%lfilled_Ind_Equivalent);inversion HLI;inversion H8;subst;simpl.
+    iApply (wp_frame_bind with "[$]");auto.
+    iIntros "Hf".
+    match goal with | |- context [ [AI_label _ _ ?l] ] => set (e:=l) end.
+    build_ctx e.
+    iApply wp_label_bind.
+    subst e.
+    iDestruct "Hv" as "[%Hcontr|Hws]";[done|iDestruct "Hws" as (ws) "[%Heq Hws]"].
+    iDestruct (big_sepL2_length with "Hws") as %Hlen. inversion Heq;subst.
+    destruct ws as [|w0 ws];[done|destruct ws as [|w1 ws];[done|destruct ws as [|w2 ws];[|done]]].
+    iSimpl in "Hws".
+    iDestruct "Hws" as "[Hw0 [Hw1 _]]".
+    iDestruct "Hw0" as (z0) "->".
+    iDestruct "Hw1" as (z1) "->".
+    pose proof (value_of_uint_repr z0) as [v ->]. iSimpl in "Hf".
+    take_drop_app_rewrite (length (validate_stack 1)).
+
+    match goal with | |- context [ (WP ?e @ _; _ {{ _ }} )%I ] => set (e0:=e) end.
+    match goal with | |- context [ (↪[frame] ?f0)%I ] => set (f':=f0) end.
+    build_ctx e0. subst e0.
+    iApply wp_seq_can_trap_ctx.
+    instantiate (1:=(λ f0, ⌜f0 = f'⌝ ∗ na_own logrel_nais ⊤)%I).
+    iFrame "Hf".
+    iSplitR;[|iSplitR;[|iSplitL]];cycle 1.
+    - iIntros (f0) "(Hf & -> & Hown)".
+      deconstruct_ctx.
+      iApply (wp_wand _ _ _ (λ v, ⌜v = trapV⌝ ∗ _)%I with "[Hf]").
+      iApply (wp_label_trap with "Hf");auto.
+      iIntros (v0) "[-> Hf]". iExists _. iFrame.
+      iIntros "Hf".
+      iApply (wp_frame_trap with "Hf").
+      iNext. iLeft. iLeft. auto.
+    - iIntros "Hf". iFrame.
+      iApply (wp_wand with "[Hf]").
+      iApply check_stack_valid;iFrame;subst;eauto.
+      iIntros (v0) "[$ HH]". eauto.
+    - subst f'. iIntros (w f0) "([-> %Hdiv] & Hf & -> & Hown) /=".
+      deconstruct_ctx.
+      take_drop_app_rewrite (length (validate_stack_bound 0)).
+      iApply fupd_wp.
+      iMod (na_inv_acc with "Hstk Hown") as "(>Hstkres & Hown & Hcls)";[solve_ndisj..|].
+      iModIntro.
+      iDestruct "Hstkres" as (l Hmul) "[Hlen Hstkres]".
+      iDestruct "Hstkres" as (l' Hmultiple) "Hl'".
+      match goal with | |- context [ (WP ?e @ _; _ {{ _ }} )%I ] => set (e0:=e) end.
+      match goal with | |- context [ (↪[frame] ?f0)%I ] => set (f':=f0) end.
+      match goal with | |- context [ (?P ={⊤}=∗ ?Q)%I ] => set (CLS:=(P ={⊤}=∗ Q)%I) end.
+      
+      set (k:=Wasm_int.N_of_uint i32m ((Wasm_int.int_of_Z i32m (Z.of_N v)))).
+      destruct (decide (k < N.of_nat l)%N).
+      + apply div_mod_i32 in Hdiv as Hdiv'.
+        eapply multiples_upto_in in Hmultiple as Hin;[..|apply Hdiv'];[|lia].
+        apply elem_of_list_lookup_1 in Hin as [i Hi].
+        iDestruct (big_sepL_lookup_acc with "Hl'") as "[Hv Hl']";[eauto|].
+        iDestruct "Hv" as (stk) "Hv".
+        iApply (wp_seq _ _ _ (λ v, ⌜v = immV []⌝ ∗ _)%I).
+        iSplitR;[by iIntros "[%Hcontr _]"|].
+        iSplitL "Hf Hv".
+        { iApply is_stack_bound_valid. iFrame "Hf Hv". iSplit;auto.
+          iPureIntro. subst f'. simpl. unfold value_of_uint.
+          f_equal. f_equal. apply int_of_Z_mod. }
+        iIntros (w) "(-> & Hstack & Hf) /=".
+        destruct (decide (N.of_nat (length stk) < two14 - 1)%N).
+        * iApply (spec_push_op with "[$Hstack $Hf]").
+          { repeat iSplit;auto. subst f';simpl. iPureIntro.
+            unfold value_of_uint. f_equal. f_equal. apply int_of_Z_mod. }
+          iIntros (w) "[-> [Hstack Hf]]".
+          iDestruct "Hf" as (f1) "[Hf %Hfeq]".
+          iDestruct ("Hl'" with "[Hstack]") as "Hl'".
+          { iExists _. iFrame. }
+          deconstruct_ctx.
+          iApply fupd_wp.
+          iMod ("Hcls" with "[Hlen Hl' $Hown]") as "Hown".
+          { iExists _. iFrame. iNext. iSplit;auto. }
+          iModIntro.
+          iApply (wp_wand _ _ _ (λ v, ⌜v = immV []⌝ ∗ _)%I with "[Hf]").
+          iApply (wp_label_value with "Hf");eauto.
+          iIntros (v0) "[-> Hf]".
+          iExists _. iFrame.
+          iIntros "Hf".
+          iApply (wp_frame_value with "Hf");eauto.
+          iNext. iLeft. iRight. iExists []. simpl. done.
+        * iDestruct (stack_pure with "Hstack") as "(_ & _ & %Hstkbound & Hstack)".
+          take_drop_app_rewrite (length (is_full_op)).
+          iApply wp_seq.
+          iSplitR;[|iSplitL "Hf Hstack"];cycle 1.
+          { iApply (spec_is_full_op with "[$Hf $Hstack]").
+            - repeat iSplit;auto.
+              iPureIntro. subst f';simpl. unfold value_of_uint.
+              f_equal. f_equal. apply int_of_Z_mod.
+            - iIntros (w) "H". iExact "H". }
+          2: iIntros "H";by iDestruct "H" as (? ?) "_".
+          iIntros (w) "H".
+          iDestruct "H" as (k0) "(-> & Hstack & [[-> %Hcond]|[-> %Hcond]] & Hf)";[|lia].
+          simpl.
+          iDestruct ("Hl'" with "[Hstack]") as "Hl'".
+          { iExists _. iFrame. }
+          iApply fupd_wp.
+          iMod ("Hcls" with "[Hlen Hl' $Hown]") as "Hown".
+          { iExists _. iFrame. iNext. iSplit;auto. }
+          iModIntro.
+          take_drop_app_rewrite 2.
+          iApply (wp_wand _ _ _ (λ v, ⌜v = trapV⌝ ∗ _)%I with "[Hf]").
+          iApply wp_seq_trap. iFrame.
+          iIntros "Hf". iApply (wp_if_true with "[$]");auto.
+          iNext. iIntros "Hf".
+          take_drop_app_rewrite 0.
+          iApply (wp_block with "[$]");auto.
+          iNext. iIntros "Hf".
+          build_ctx [AI_basic BI_unreachable].
+          take_drop_app_rewrite 1.
+          iApply wp_seq_trap_ctx. iFrame. iIntros "Hf".
+          iApply (wp_unreachable with "[$]"). auto.
+          iIntros (v') "[-> Hf]".
+          deconstruct_ctx.
+          iApply (wp_wand _ _ _ (λ v, ⌜v = trapV⌝ ∗ _)%I with "[Hf]").
+          iApply (wp_label_trap with "[$]");eauto.
+          iIntros (v0) "[-> Hf]".
+          iExists _. iFrame. iIntros "Hf".
+          iApply (wp_frame_trap with "[$]").
+          iNext. iLeft. iLeft. auto.          
+      + iApply (wp_wand with "[Hlen Hf]").
+        iApply (fail_stack_bound_valid with "[$Hlen $Hf]").
+        eauto.
+        iIntros (v0) "(-> & Hlen & Hf)".
+        deconstruct_ctx.
+        iApply fupd_wp.
+        iMod ("Hcls" with "[$Hown Hl' Hlen]") as "Hown".
+        { iNext. iExists _. iFrame. auto. }
+        iModIntro.
+        iApply (wp_wand _ _ _ (λ v, ⌜v = trapV⌝ ∗ _)%I with "[Hf]").
+        iApply (wp_label_trap with "Hf");eauto.
+        iIntros (v0) "[-> Hf]".
+        iExists _. iFrame. iIntros "Hf".
+        iApply (wp_frame_trap with "[$]").
+        iNext. iLeft. iLeft. auto.
+    - iIntros "[%Hcontr _]";done.
+  Qed.
+*)
+    
+  End valid.
+
+End stack.    
+
